ebpf/Mulh.v
@@ -1,0 +1,141 @@
+(* *********************************************************************)
+(*           Emulation of mulhs, mulhu                                 *)
+(*       Frédéric Besson (frederic.besson@inria.fr), Inria Rennes      *)
+(* *********************************************************************)
+
+Require Import Coqlib Errors Maps.
+Require Import AST Zbits Integers Floats Values Memory Globalenvs.
+
+Definition mulhu' (x y:Int.int) : Int.int :=
+  Int64.hiword (Int64.mul (Int64.repr (Int.unsigned x)) (Int64.repr (Int.unsigned y))).
+
+Definition mulhs' (x y:Int.int) : Int.int :=
+  Int64.hiword (Int64.mul (Int64.repr (Int.signed x)) (Int64.repr (Int.signed y))).
+
+#[ global] Hint Resolve Int64.int_unsigned_range : mulh.
+
+Lemma int64_max_unsigned_pos : Int64.max_unsigned > 0.
+Proof.
+  compute; congruence.
+Qed.
+
+#[ global] Hint Resolve int64_max_unsigned_pos : mulh.
+
+Lemma unsigned_repr_int_unsigned : forall x,
+    Int64.unsigned (Int64.repr (Int.unsigned x)) = Int.unsigned x.
+Proof.
+  intros.
+  rewrite Int64.unsigned_repr; auto with mulh.
+Qed.
+
+Lemma signed_repr_int_signed : forall x,
+    Int64.signed (Int64.repr (Int.signed x)) = Int.signed x.
+Proof.
+  intros. rewrite Int64.signed_repr;auto.
+  generalize (Int.signed_range x).
+  assert (Int64.min_signed <= Int.min_signed).
+  { compute. congruence. }
+    assert (Int.max_signed <= Int64.max_signed).
+  { compute. congruence. }
+  lia.
+Qed.
+
+Lemma mulhu_eq : forall x y, Int.mulhu x y = mulhu' x y.
+Proof.
+  unfold Int.mulhu, mulhu'.
+  intros. unfold Int64.hiword.
+  symmetry.
+  f_equal.
+  rewrite Int64.shru_div_two_p.
+  change (two_p (Int64.unsigned (Int64.repr Int.zwordsize))) with (Int.modulus).
+  assert (MULB : 0 <= Int.unsigned x * Int.unsigned y <= Int64.max_unsigned).
+  {
+    generalize (Int.unsigned_range_2 x).
+    generalize (Int.unsigned_range_2 y).
+    assert (Int.max_unsigned * Int.max_unsigned <= Int64.max_unsigned).
+    { compute. congruence. }
+    nia.
+  }
+  unfold Int64.mul.
+  rewrite! Int64.unsigned_repr;auto with mulh;
+    rewrite! Int64.unsigned_repr; auto with mulh.
+  { apply Zdiv_interval_2;auto.
+    lia. generalize int64_max_unsigned_pos; lia.
+    apply Int.modulus_pos.
+  }
+  rewrite! unsigned_repr_int_unsigned; auto.
+Qed.
+
+Lemma hiword_shrl : forall i, Int64.hiword i = Int64.loword (Int64.shr' i (Int.repr 32)).
+Proof.
+  intros.
+  apply Int.same_bits_eq.
+  intros.
+  rewrite Int64.bits_hiword by auto.
+  rewrite Int64.bits_loword by auto.
+  assert (LT : 2 * Int.zwordsize = Int64.zwordsize) by (compute; congruence).
+  rewrite Int64.bits_shr' by lia.
+  destruct (zlt (i0 + Int.unsigned (Int.repr 32)) Int64.zwordsize).
+  reflexivity.
+  change (Int.unsigned (Int.repr 32)) with Int.zwordsize in g.
+  lia.
+Qed.
+
+Lemma zmod_small_add : forall a b,
+    0 <= a + b < b ->
+    a mod b = a + b.
+Proof.
+  intros.
+  rewrite <- (Z_mod_plus_full a 1).
+  rewrite Zmod_small. ring.
+  lia.
+Qed.
+
+Lemma signed_unsigned_diff0 : forall x,
+    Int.signed x <> 0 -> Int.unsigned x <> 0.
+Proof.
+  intros.
+  intro.
+  unfold Int.signed in H.
+  destruct (zlt (Int.unsigned x) Int.half_modulus).
+  tauto. generalize Int.half_modulus_pos. lia.
+Qed.
+
+
+Lemma mulhs_eq : forall x y, Int.mulhs x y = mulhs' x y.
+Proof.
+  unfold Int.mulhs, mulhs'.
+  intros.
+  unfold Int64.hiword.
+  rewrite Int64.shru_div_two_p.
+  change (two_p (Int64.unsigned (Int64.repr Int.zwordsize))) with (Int.modulus).
+  rewrite Int64.mul_signed.
+  rewrite! signed_repr_int_signed.
+  rewrite Int64.unsigned_repr.
+  {
+    rewrite Int64.unsigned_repr_eq.
+    destruct (Z.eq_dec (Int.signed x) 0) as [ZX |NZX].
+    rewrite ZX. reflexivity.
+    destruct (Z.eq_dec (Int.signed y) 0) as [ZY |NZY].
+    rewrite ZY. rewrite Z.mul_0_r. reflexivity.
+    apply signed_unsigned_diff0 in NZX.
+    apply signed_unsigned_diff0 in NZY.
+    apply Int.same_bits_eq. intros.
+    rewrite! Int.testbit_repr by auto.
+    change Int.modulus with (2^32).
+    change Int64.modulus with (2^64).
+    rewrite Z.div_pow2_bits  by lia.
+    rewrite Z.div_pow2_bits  by lia.
+    rewrite Z.testbit_mod_pow2 by lia.
+    destruct (i + 32 <? 64) eqn:LT.
+    reflexivity.
+    simpl.
+    rewrite Z.ltb_ge in LT.
+    change Int.zwordsize with 32 in H. lia.
+  }
+  { apply Zdiv_interval_2;auto.
+    apply Int64.unsigned_range_2.
+    lia. generalize int64_max_unsigned_pos;lia.
+    apply Int.modulus_pos.
+  }
+Qed.
